<?xml version="1.0" encoding="UTF-8"?>
<!DOCTYPE rdf:RDF>
<rdf:RDF xmlns:rdf="http://www.w3.org/1999/02/22-rdf-syntax-ns#"
         xmlns:rdfs="http://www.w3.org/2000/01/rdf-schema#"
         xmlns:owl="http://www.w3.org/2002/07/owl#"
         xmlns:dc="http://purl.org/dc/elements/1.1/"
         xmlns:dcterms="http://purl.org/dc/terms/"
         xmlns:vs="http://www.w3.org/2003/06/sw-vocab-status/ns#"
         xmlns:capability="http://www.science.uva.nl/research/sne/ndl/capability#"
>

<rdf:Description rdf:about="http://www.science.uva.nl/research/sne/ndl/capability#">
    <rdfs:isDefinedBy rdf:resource="http://www.science.uva.nl/research/sne/schema/capability.rdf"/>
    <rdf:type rdf:resource="http://www.w3.org/2002/07/owl#Ontology"/>
    <rdfs:label>ndlcap</rdfs:label>
    <dc:title xml:lang="en">Network Description Language: Network Device Capability module</dc:title>
    <dc:description xml:lang="en">A vocabulary for defining dynamic capabilities of a network device.</dc:description>
    <dc:publisher xml:lang="en">System and Network Engineering group, Universiteit van Amsterdam</dc:publisher>
    <dcterms:issued>2006-12-05</dcterms:issued>
    <dcterms:modified>2007-01-21</dcterms:modified>
    <owl:versionInfo>2.4</owl:versionInfo>
    <vs:term_status>testing</vs:term_status>
    <vs:userdocs rdf:resource="http://www.science.uva.nl/research/sne/ndl/?c=13-Capability-Schema"/>
    <vs:moreinfo>WARNING: This schema has testing status and is extremely likely to change! Please wait at least wait till it is in unstable mode before using it. Hopefully, some of it's concepts will crystalize, and get incorporated in some of the ideas put forward in the NML workgroup in the OGF (www.ogf.org).</vs:moreinfo>
</rdf:Description>

<!-- Classes -->

<rdfs:Class rdf:about="http://www.science.uva.nl/research/sne/ndl/capability#SwitchMatrix">
    <rdfs:isDefinedBy rdf:resource="http://www.science.uva.nl/research/sne/schema/capability.rdf"/>
    <rdfs:label xml:lang="en">Switch Matrix</rdfs:label>
    <rdfs:comment xml:lang="en">A network element(s) that can be represented as a subnetwork (ITU-T G.805 terminology). Typically the switching core within a device.</rdfs:comment>
    <vs:moreinfo>WARNING: It is not yet clear if a switch matrix is an actual instance within each device, or merely a representation of a certain kind of switch matrix.</vs:moreinfo>
    <rdfs:subClassOf rdf:resource="http://www.science.uva.nl/research/sne/ndl#NetworkElement"/>
</rdfs:Class>

<rdfs:Class rdf:about="http://www.science.uva.nl/research/sne/ndl/capability#PotentialInterface">
    <rdfs:isDefinedBy rdf:resource="http://www.science.uva.nl/research/sne/schema/capability.rdf"/>
    <rdfs:label xml:lang="en">Potential Interface</rdfs:label>
    <rdfs:comment xml:lang="en">An abstract interface, which could be created as the result of a adaptation capability present in an actual server or client interface.</rdfs:comment>
    <rdfs:subClassOf rdf:resource="http://www.science.uva.nl/research/sne/ndl#ConnectionPoint"/>
</rdfs:Class>

<rdfs:Class rdf:about="http://www.science.uva.nl/research/sne/capability#InstantiatedMuxInterface">
    <rdfs:isDefinedBy rdf:resource="http://www.science.uva.nl/research/sne/schema/capability.rdf"/>
    <rdfs:label xml:lang="en">Instantiated Interface</rdfs:label>
    <rdfs:comment xml:lang="en">An Interface, which is an instantiated of a potential interface. it exists now, but can be removed; the use of this type instead of the Interface class simply means that this data is considered more dynamic, and should not be cached for a longer time. It does not define a strict time-scale.</rdfs:comment>
    <rdfs:subClassOf rdf:resource="http://www.science.uva.nl/research/sne/ndl#ConnectionPoint"/>
    <rdfs:subClassOf rdf:resource="http://www.science.uva.nl/research/sne/ndl#Interface"/>
    <rdfs:subClassOf rdf:resource="http://www.science.uva.nl/research/sne/ndl#NetworkElement"/>
</rdfs:Class>

<rdfs:Class rdf:about="http://www.science.uva.nl/research/sne/ndl/capability#CastType">
    <rdfs:isDefinedBy rdf:resource="http://www.science.uva.nl/research/sne/schema/capability.rdf"/>
    <rdfs:label xml:lang="en">Casting Type</rdfs:label>
    <rdfs:comment>The cast (unicast/multicast/broadcast) type to specify the internal switching type.</rdfs:comment>
</rdfs:Class>

<!-- Resources -->

<capability:CastType rdf:about="http://www.science.uva.nl/research/sne/ndl/capability#Unicast">
    <rdfs:isDefinedBy rdf:resource="http://www.science.uva.nl/research/sne/schema/capability.rdf"/>
    <rdfs:label xml:lang="en">Unicast</rdfs:label>
    <rdfs:comment xml:lang="en">The Switch Matrix is capable of creating a switched to between object and subject Interface if no other switchedTo exist with the same object, and no other switchedTo exist with the same subject.</rdfs:comment>
</capability:CastType>

<capability:CastType rdf:about="http://www.science.uva.nl/research/sne/ndl/capability#Multicast">
    <rdfs:isDefinedBy rdf:resource="http://www.science.uva.nl/research/sne/schema/capability.rdf"/>
    <rdfs:label xml:lang="en">Multicast</rdfs:label>
    <rdfs:comment xml:lang="en">The Switch Matrix is capable of creating a switched to between any object and subject Interface, regardless of existing switched to properties.</rdfs:comment>
</capability:CastType>

<capability:CastType rdf:about="http://www.science.uva.nl/research/sne/ndl/capability#Broadcast">
    <rdfs:isDefinedBy rdf:resource="http://www.science.uva.nl/research/sne/schema/capability.rdf"/>
    <rdfs:label xml:lang="en">Broadcast</rdfs:label>
    <rdfs:comment xml:lang="en">The Switch Matrix has a switchedTo between an object and subject Interface if and only if the object and subject interface have the same label property.</rdfs:comment>
</capability:CastType>

<!--
<capability:CastType rdf:about="http://www.science.uva.nl/research/sne/ndl/capability#AltSwitch">
    <rdfs:isDefinedBy rdf:resource="http://www.science.uva.nl/research/sne/schema/capability.rdf"/>
    <rdfs:label xml:lang="en">AltSwitch</rdfs:label>
    <rdfs:comment xml:lang="en">The Switch Matrix is capable of creating an altSwitchedTo properties besides regular switchedTo properties. AltSwitchedTo are used for backup paths, where the object Interface of multiple altSwitchedTo properties chooses which data to carry forward, based on the strongest signal. A regular switchedTo would mean that the data is somehow merged.</rdfs:comment>
    <vs:moreinfo>It is not clear if the "CastType" is the best way to assign this value to a SwitchingMatrix. We may use a dedicated type for back up connections.</vs:moreinfo>
</capability:CastType>
-->

<!-- Predicates -->

<rdf:Property rdf:about="http://www.science.uva.nl/research/sne/ndl/capability#internalLabel">
    <rdfs:isDefinedBy rdf:resource="http://www.science.uva.nl/research/sne/schema/capability.rdf"/>
    <rdfs:label xml:lang="en">internal label</rdfs:label>
    <rdfs:comment>The internal label of the Interface, which is required for the switching capability and swapping capability of a Switch Matrix. As the internal label is a subProperty of te label property, if a label property is set, then the internal label has that same value. Only in rare conditions is the internal label set, but the regular label not. Untagged Ethernet VLANs are the only technology we're aware of where this is the case.</rdfs:comment>
    <rdfs:domain rdf:resource="http://www.science.uva.nl/research/sne/ndl#Interface"/>
    <rdfs:range rdf:resource="http://www.w3.org/2000/01/rdf-schema#Literal"/>
    <rdfs:subPropertyOf rdf:resource="http://www.science.uva.nl/research/sne/ndl/layer#label"/>
    <rdfs:subPropertyOf rdf:resource="http://www.science.uva.nl/research/sne/ndl/layer#property"/>
</rdf:Property>

<rdf:Property rdf:about="http://www.science.uva.nl/research/sne/ndl/capability#hasSwitchMatrix">
    <rdfs:isDefinedBy rdf:resource="http://www.science.uva.nl/research/sne/schema/capability.rdf"/>
    <rdfs:label xml:lang="en">has switch matrix</rdfs:label>
    <rdfs:comment xml:lang="en">Couples a particular switch matrix to a device.</rdfs:comment>
    <rdfs:seeAlso rdf:resource="http://www.science.uva.nl/research/sne/ndl/capability#swappingCapability"/>
    <rdfs:domain rdf:resource="http://www.science.uva.nl/research/sne/ndl#Device"/>
    <rdfs:range rdf:resource="http://www.science.uva.nl/research/sne/ndl/capability#SwitchMatrix"/>
</rdf:Property>

<rdf:Property rdf:about="http://www.science.uva.nl/research/sne/ndl/capability#inMatrix">
    <rdfs:isDefinedBy rdf:resource="http://www.science.uva.nl/research/sne/schema/capability.rdf"/>
    <rdfs:label xml:lang="en">in matrix</rdfs:label>
    <rdfs:comment xml:lang="en">Couples a particular interface to a switch matrix.</rdfs:comment>
    <rdfs:domain rdf:resource="http://www.science.uva.nl/research/sne/ndl#ConnectionPoint"/>
    <rdfs:range rdf:resource="http://www.science.uva.nl/research/sne/ndl/capability#SwitchMatrix"/>
</rdf:Property>

<rdf:Property rdf:about="http://www.science.uva.nl/research/sne/ndl/capability#switchingCapability">
    <rdfs:isDefinedBy rdf:resource="http://www.science.uva.nl/research/sne/schema/capability.rdf"/>
    <rdfs:label xml:lang="en">switching capability</rdfs:label>
    <rdfs:comment xml:lang="en">A device is capable of dynamically forwarding (switching) data based on the (value of the) internal label property of the object Interface to any other Interface of the same type, provided that the value of the label of both Interfaces are equal. Two empty labels are considered equal. For example, an Ethernet device is able to forward data from an Ethernet Interface 2 with VLAN (802.1Q) label "23" to Ethernet Interface 3 with the same VLAN label ("23"). A device which statically forwards data, like a patch panel, should NOT have the switching capability defined. A SwitchMatrix can only have one switchingCapability. A device can have multiple SwitchMatrices.</rdfs:comment>
    <rdfs:seeAlso rdf:resource="http://www.science.uva.nl/research/sne/ndl/capability#swappingCapability"/>
    <rdfs:domain rdf:resource="http://www.science.uva.nl/research/sne/ndl/capability#SwitchMatrix"/>
    <rdfs:range rdf:resource="http://www.science.uva.nl/research/sne/ndl/layer#Layer"/>
    <vs:moreinfo>WARNING: The switchingCapability used to be defined for a Device, but that was changed to SwitchMatrix.</vs:moreinfo>
</rdf:Property>

<rdf:Property rdf:about="http://www.science.uva.nl/research/sne/ndl/capability#swappingCapability">
    <rdfs:isDefinedBy rdf:resource="http://www.science.uva.nl/research/sne/schema/capability.rdf"/>
    <rdfs:label xml:lang="en">swapping capability</rdfs:label>
    <rdfs:comment xml:lang="en">A device is capable of dynamically forwarding (switching) data based on the (value of the) internal label property of the object Interface to any other Interface of the same type, provided that the value of the label of both Interfaces are different. Two empty labels are considered equal. For example, AAL0 Interface 38 with label VCI 23 is capable of forwarding data to AAL0 Interface 17, with VCI 18. Usually, a device with swapping capability also has switching capability. A SwitchMatrix can only have one swappingCapability. A device can have multiple SwitchMatrices.</rdfs:comment>
    <rdfs:seeAlso rdf:resource="http://www.science.uva.nl/research/sne/ndl/capability#switchingCapability"/>
    <rdfs:domain rdf:resource="http://www.science.uva.nl/research/sne/ndl/capability#SwitchMatrix"/>
    <rdfs:range rdf:resource="http://www.science.uva.nl/research/sne/ndl/layer#Layer"/>
    <vs:moreinfo>WARNING: The switchingCapability used to be defined for a Device, but that was changed to SwitchMatrix.</vs:moreinfo>
</rdf:Property>

<rdf:Property rdf:about="http://www.science.uva.nl/research/sne/ndl/capability#hasCastType">
    <rdfs:isDefinedBy rdf:resource="http://www.science.uva.nl/research/sne/schema/capability.rdf"/>
    <rdfs:label xml:lang="en">has cast type</rdfs:label>
    <rdfs:comment xml:lang="en">The casting type of a Switch Matrix, explaining which switchedTo connections van be made by the Switch Matrix.</rdfs:comment>
    <rdfs:seeAlso rdf:resource="http://www.science.uva.nl/research/sne/ndl/capability#swappingCapability"/>
    <rdfs:domain rdf:resource="http://www.science.uva.nl/research/sne/ndl/capability#SwitchMatrix"/>
    <rdfs:range rdf:resource="http://www.science.uva.nl/research/sne/ndl/capability#CastType"/>
</rdf:Property>

<rdf:Property rdf:about="http://www.science.uva.nl/research/sne/ndl/capability#memoryBuffer">
    <rdfs:isDefinedBy rdf:resource="http://www.science.uva.nl/research/sne/schema/capability.rdf"/>
    <rdfs:label xml:lang="en">memory buffer</rdfs:label>
    <rdfs:comment xml:lang="en">The size of the internal memory buffer of the Switch Matrix.</rdfs:comment>
    <rdfs:seeAlso rdf:resource="http://www.science.uva.nl/research/sne/ndl/capability#swappingCapability"/>
    <rdfs:domain rdf:resource="http://www.science.uva.nl/research/sne/ndl/capability#SwitchMatrix"/>
    <rdfs:range rdf:resource="http://www.w3.org/2001/XMLSchema#float"/>
</rdf:Property>

<rdf:Property rdf:about="http://www.science.uva.nl/research/sne/ndl/capability#capacities">
    <rdfs:isDefinedBy rdf:resource="http://www.science.uva.nl/research/sne/schema/capability.rdf"/>
    <rdfs:label xml:lang="en">capacities</rdfs:label>
    <rdfs:comment xml:lang="en">The potential interface can take any of the given capacities. The range is a RDF:Alt, each containing a float with the capacity in Byte/s.</rdfs:comment>
    <rdfs:seeAlso rdf:resource="http://www.science.uva.nl/research/sne/ndl#capacity"/>
    <rdfs:domain rdf:resource="http://www.science.uva.nl/research/sne/ndl#ConnectionPoint"/>
    <rdfs:range rdf:resource="http://www.w3.org/1999/02/22-rdf-syntax-ns#Alt"/>
</rdf:Property>

<rdf:Property rdf:about="http://www.science.uva.nl/research/sne/ndl/capability#labels">
    <rdfs:isDefinedBy rdf:resource="http://www.science.uva.nl/research/sne/schema/capability.rdf"/>
    <rdfs:label xml:lang="en">labels</rdfs:label>
    <rdfs:comment xml:lang="en">The interface can potentially take any of these labels.</rdfs:comment>
    <rdfs:domain rdf:resource="http://www.science.uva.nl/research/sne/ndl#ConnectionPoint"/>
    <rdfs:range rdf:resource="http://www.science.uva.nl/research/sne/ndl/layer#LabelSet"/>
</rdf:Property>

<rdf:Property rdf:about="http://www.science.uva.nl/research/sne/ndl/capability#properties">
    <rdfs:isDefinedBy rdf:resource="http://www.science.uva.nl/research/sne/schema/capability.rdf"/>
    <rdfs:label xml:lang="en">encoding properties</rdfs:label>
    <rdfs:comment xml:lang="en">The interface is able to configure one or more of the given encoding properties. The range is either a RDF:Alt of properties if the Interface can only configure one encoding property at the same time, or a RDF:Bag of encoding properties if the Interface can configure multiple encoding properties at the same time.</rdfs:comment>
    <rdfs:domain rdf:resource="http://www.science.uva.nl/research/sne/ndl#Interface"/>
    <rdfs:range rdf:resource="http://www.w3.org/2000/01/rdf-schema#Container"/>
    <rdfs:seeAlso rdf:resource="http://www.science.uva.nl/research/sne/ndl/layer#property"/>
</rdf:Property>

<rdf:Property rdf:about="http://www.science.uva.nl/research/sne/ndl/capability#ingressProperties">
    <rdfs:isDefinedBy rdf:resource="http://www.science.uva.nl/research/sne/schema/capability.rdf"/>
    <rdfs:label xml:lang="en">ingress encoding properties</rdfs:label>
    <rdfs:comment xml:lang="en">The interface is able to configure one or more of the given ingress encoding properties. The range is either a RDF:Alt of properties if the Interface can only configure one ingress encoding property at the same time, or a RDF:Bag of encoding properties if the Interface can configure multiple ingress encoding properties at the same time.</rdfs:comment>
    <rdfs:domain rdf:resource="http://www.science.uva.nl/research/sne/ndl#Interface"/>
    <rdfs:range rdf:resource="http://www.w3.org/2000/01/rdf-schema#Container"/>
    <rdfs:seeAlso rdf:resource="http://www.science.uva.nl/research/sne/ndl/layer#ingressProperty"/>
</rdf:Property>

<rdf:Property rdf:about="http://www.science.uva.nl/research/sne/ndl/capability#egressProperties">
    <rdfs:isDefinedBy rdf:resource="http://www.science.uva.nl/research/sne/schema/capability.rdf"/>
    <rdfs:label xml:lang="en">egress encoding properties</rdfs:label>
    <rdfs:comment xml:lang="en">The interface is able to configure one or more of the given egres  encoding properties. The range is either a RDF:Alt of properties if the Interface can only configure one egress encoding property at the same time, or a RDF:Bag of encoding properties if the Interface can configure multiple egress encoding properties at the same time.</rdfs:comment>
    <rdfs:domain rdf:resource="http://www.science.uva.nl/research/sne/ndl#Interface"/>
    <rdfs:range rdf:resource="http://www.w3.org/2000/01/rdf-schema#Container"/>
    <rdfs:seeAlso rdf:resource="http://www.science.uva.nl/research/sne/ndl/layer#egressProperty"/>
</rdf:Property>

<!--
Possible more adaptation function properties:
- interworking of adaptation
-->

</rdf:RDF>