<?xml version="1.0" encoding="UTF-8"?>
<!DOCTYPE rdf:RDF>
<rdf:RDF xmlns:rdf="http://www.w3.org/1999/02/22-rdf-syntax-ns#"
         xmlns:rdfs="http://www.w3.org/2000/01/rdf-schema#"
         xmlns:owl="http://www.w3.org/2002/07/owl#"
         xmlns:dc="http://purl.org/dc/elements/1.1/"
         xmlns:dcterms="http://purl.org/dc/terms/"
         xmlns:vs="http://www.w3.org/2003/06/sw-vocab-status/ns#"
         xmlns:ndl="http://www.science.uva.nl/research/sne/ndl#"
         xmlns:layer="http://www.science.uva.nl/research/sne/ndl/layer#"
         xmlns:wireless="http://www.science.uva.nl/research/sne/ndl/wireless#"
>

<rdf:Description rdf:about="http://www.science.uva.nl/research/sne/ndl/wireless#">
    <rdfs:isDefinedBy rdf:resource="http://www.science.uva.nl/research/sne/schema/wireless.rdf"/>
    <rdf:type rdf:resource="http://www.w3.org/2002/07/owl#Ontology"/>
    <rdfs:label>wireless</rdfs:label>
    <dc:title xml:lang="en">Network Description Language: Wireless technologies</dc:title>
    <dc:description xml:lang="en">A vocabulary for defining a wireless network. This schema only defines the 802.11 layer. It could easily be extended to support other wireless layers.</dc:description>
    <dc:publisher xml:lang="en">System and Network Engineering group, Universiteit van Amsterdam</dc:publisher>
    <dcterms:issued>2007-01-21</dcterms:issued>
    <dcterms:modified>2007-01-21</dcterms:modified>
    <owl:versionInfo>2.4</owl:versionInfo>
    <vs:term_status>testing</vs:term_status>
    <vs:userdocs rdf:resource="http://www.science.uva.nl/research/sne/ndl/?c=20-Technology-Schemas"/>
    <vs:moreinfo>WARNING: this schema is merely an example what can be done with the layer schema. It was never meant for serious usage. For that, look at the output of the NML workgroup in the OGF (www.ogf.org). We regard this schema in particular as a "quick hack". We're not experts in the technologies mentioned here, and will likely have overlooked a few things. Feel free to make a schema for these technologies based on our layer schema, or (slightly) better example schemas (e.g. Ethernet, TDM or WDM), but please start from scratch for this particular technology.</vs:moreinfo>
</rdf:Description>

<!-- TWISTED PAIR LAYER -->

<!-- Classes -->

<rdfs:Class rdf:about="http://www.science.uva.nl/research/sne/ndl/wireless#IEEE802-11NetworkElement">
    <rdfs:isDefinedBy rdf:resource="http://www.science.uva.nl/research/sne/schema/wireless.rdf"/>
    <rdfs:label xml:lang="en">802.11</rdfs:label>
    <rdfs:comment xml:lang="en">Network Elements on the 802.11 Layer. This encompasses all 802.11 standards. This layer is modeled a packet switched broadcast network, much like TaggedEthernet, and has the SSID as the basic switching label. The modeling does not fit well, as it only has a rudimentary concept of signal strengths. This could probably be improved by creating two layers: one for each SSID, and one for each pair of transmitter and receiver.</rdfs:comment>
    <rdf:type rdf:resource="http://www.science.uva.nl/research/sne/ndl/layer#Layer"/>
    <rdfs:subClassOf rdf:resource="http://www.science.uva.nl/research/sne/ndl#NetworkElement"/>
</rdfs:Class>

<!--
<rdfs:Class rdf:about="http://www.science.uva.nl/research/sne/ndl/wireless#IEEE802-11Interface">
    <rdfs:isDefinedBy rdf:resource="http://www.science.uva.nl/research/sne/schema/wireless.rdf"/>
    <rdfs:label xml:lang="en">802.11</rdfs:label>
    <rdf:type rdf:resource="http://www.science.uva.nl/research/sne/ndl/layer#InterfaceClass"/>
    <rdfs:subClassOf rdf:resource="http://www.science.uva.nl/research/sne/ndl#ConnectionPoint"/>
    <rdfs:subClassOf rdf:resource="http://www.science.uva.nl/research/sne/ndl/wireless#IEEE802-11NetworkElement"/>
</rdfs:Class>
-->

<rdfs:Class rdf:about="http://www.science.uva.nl/research/sne/ndl/wireless#IEEE802-11Standard">
    <rdfs:isDefinedBy rdf:resource="http://www.science.uva.nl/research/sne/schema/wireless.rdf"/>
    <rdfs:label xml:lang="en">Shielding</rdfs:label>
    <rdfs:comment xml:lang="en">The shielding of the wireless pairs in a cable.</rdfs:comment>
</rdfs:Class>

<rdfs:Class rdf:about="http://www.science.uva.nl/research/sne/ndl/wireless#AccessSecurity">
    <rdfs:isDefinedBy rdf:resource="http://www.science.uva.nl/research/sne/schema/wireless.rdf"/>
    <rdfs:label xml:lang="en">AccessSecurity</rdfs:label>
    <rdfs:comment xml:lang="en">The encryption used to authenticate to a base station.</rdfs:comment>
</rdfs:Class>

<!-- Resources -->

<wireless:IEEE802-11Standard rdf:about="http://www.science.uva.nl/research/sne/ndl/wireless#IEEE802-11b">
    <rdfs:isDefinedBy rdf:resource="http://www.science.uva.nl/research/sne/schema/wireless.rdf"/>
    <rdfs:label xml:lang="en">802.11b</rdfs:label>
    <rdfs:comment xml:lang="en">IEEE 802.11b standard. 802.11b operates between 2.4 an 2.5 GHz, and has a maximum data rate of 11 Mb/s.</rdfs:comment>
</wireless:IEEE802-11Standard>

<wireless:IEEE802-11Standard rdf:about="http://www.science.uva.nl/research/sne/ndl/wireless#IEEE802-11a">
    <rdfs:isDefinedBy rdf:resource="http://www.science.uva.nl/research/sne/schema/wireless.rdf"/>
    <rdfs:label xml:lang="en">802.11a</rdfs:label>
    <rdfs:comment xml:lang="en">IEEE 802.11a standard. 802.11a operates between 5.1 an 5.9 GHz, and has a maximum data rate of 54 Mb/s. Due to the high frequency, it does not easily penetrate walls.</rdfs:comment>
</wireless:IEEE802-11Standard>

<wireless:IEEE802-11Standard rdf:about="http://www.science.uva.nl/research/sne/ndl/wireless#IEEE802-11g">
    <rdfs:isDefinedBy rdf:resource="http://www.science.uva.nl/research/sne/schema/wireless.rdf"/>
    <rdfs:label xml:lang="en">802.11g</rdfs:label>
    <rdfs:comment xml:lang="en">IEEE 802.11g standard. 802.11g operates between 2.4 and 2.5 GHz, and has a maximum data rate of 54 Mb/s.</rdfs:comment>
</wireless:IEEE802-11Standard>

<wireless:IEEE802-11Standard rdf:about="http://www.science.uva.nl/research/sne/ndl/wireless#IEEE802-11n">
    <rdfs:isDefinedBy rdf:resource="http://www.science.uva.nl/research/sne/schema/wireless.rdf"/>
    <rdfs:label xml:lang="en">802.11n</rdfs:label>
    <rdfs:comment xml:lang="en">IEEE 802.11n standard. 802.11n operates at the 2.4 GHz or 5 GHz bands, and has a maximum data rate of 540 Mb/s.</rdfs:comment>
</wireless:IEEE802-11Standard>

<wireless:AccessSecurity rdf:about="http://www.science.uva.nl/research/sne/ndl/wireless#WEP">
    <rdfs:isDefinedBy rdf:resource="http://www.science.uva.nl/research/sne/schema/wireless.rdf"/>
    <rdfs:label xml:lang="en">WEP</rdfs:label>
    <rdfs:comment xml:lang="en">Wired Equivalent Privacy (WEP). WEP uses the RC4 stream cipher.</rdfs:comment>
</wireless:AccessSecurity>

<wireless:AccessSecurity rdf:about="http://www.science.uva.nl/research/sne/ndl/wireless#WPA">
    <rdfs:isDefinedBy rdf:resource="http://www.science.uva.nl/research/sne/schema/wireless.rdf"/>
    <rdfs:label xml:lang="en">WPA</rdfs:label>
    <rdfs:comment xml:lang="en">Wi-Fi Protected Access(WPA). WPA uses the RC4 stream cipher.</rdfs:comment>
</wireless:AccessSecurity>

<wireless:AccessSecurity rdf:about="http://www.science.uva.nl/research/sne/ndl/wireless#WPA2">
    <rdfs:isDefinedBy rdf:resource="http://www.science.uva.nl/research/sne/schema/wireless.rdf"/>
    <rdfs:label xml:lang="en">WPA2</rdfs:label>
    <rdfs:comment xml:lang="en">IEEE 802.11i access encryption, also known as WPA2. WPA2 uses the AES block cipher.</rdfs:comment>
</wireless:AccessSecurity>

<rdfs:Class rdf:about="http://www.science.uva.nl/research/sne/ndl/wireless#SSIDLabel">
    <rdfs:isDefinedBy rdf:resource="http://www.science.uva.nl/research/sne/schema/wireless.rdf"/>
    <rdfs:label xml:lang="en">SSID</rdfs:label>
    <rdfs:comment xml:lang="en">The service set identifier (SSID), identifying packets on a wireless network to belong to a certain network. The SSID is a case-senstive string of up to 32 alphanumeric characters. Since xsd:string is also case-senstive, we can simply use the XML string comparison.</rdfs:comment>
    <rdf:type rdf:resource="http://www.science.uva.nl/research/sne/ndl/layer#LabelType"/>
    <rdfs:subClassOf rdf:resource="http://www.w3.org/2001/XMLSchema#string"/>
    <vs:moreinfo>The range is a 32-char alphanumeric case-sensitive string. This should be specified. Perhaps using OWL 1.1 or XSD facets. However, neither is standardized yet.</vs:moreinfo>
</rdfs:Class>

<!-- Predicates -->

<rdf:Property rdf:about="http://www.science.uva.nl/research/sne/ndl/wireless#ssid">
    <rdfs:isDefinedBy rdf:resource="http://www.science.uva.nl/research/sne/schema/wireless.rdf"/>
    <rdfs:label xml:lang="en">SSID</rdfs:label>
    <rdfs:comment xml:lang="en">The service set identifier (SSID), identifying packets on a wireless network to belong to a certain network. The SSID is a case-senstive string of up to 32 alphanumeric characters.</rdfs:comment>
    <rdfs:subPropertyOf rdf:resource="http://www.science.uva.nl/research/sne/ndl/layer#label"/>
    <rdfs:domain rdf:resource="http://www.science.uva.nl/research/sne/ndl#ConnectionPoint"/>
    <rdfs:domain rdf:resource="http://www.science.uva.nl/research/sne/ndl/wireless#IEEE802-11NetworkElement"/>
    <rdfs:range rdf:resource="http://www.science.uva.nl/research/sne/ndl/wireless#SSIDLabel"/>
    <!-- WARNING: cardinality is not sepcified according to the standard, but very easy to parse for now -->
    <owl:minCardinality rdf:datatype="http://www.w3.org/2001/XMLSchema#integer">0</owl:minCardinality> <!-- label MAY be unset for this layer -->
    <owl:maxCardinality rdf:datatype="http://www.w3.org/2001/XMLSchema#integer">1</owl:maxCardinality>
</rdf:Property>

<rdf:Property rdf:about="http://www.science.uva.nl/research/sne/ndl/wireless#standard">
    <rdfs:isDefinedBy rdf:resource="http://www.science.uva.nl/research/sne/schema/wireless.rdf"/>
    <rdfs:label xml:lang="en">standard</rdfs:label>
    <rdfs:comment xml:lang="en">The wireless standard used in the SSID network.</rdfs:comment>
    <rdfs:subPropertyOf rdf:resource="http://www.science.uva.nl/research/sne/ndl/layer#property"/>
    <rdfs:domain rdf:resource="http://www.science.uva.nl/research/sne/ndl#ConnectionPoint"/>
    <rdfs:domain rdf:resource="http://www.science.uva.nl/research/sne/ndl/wireless#IEEE802-11NetworkElement"/>
    <rdfs:range rdf:resource="http://www.science.uva.nl/research/sne/ndl/wireless#IEEE802-11Standard"/>
</rdf:Property>

<rdf:Property rdf:about="http://www.science.uva.nl/research/sne/ndl/wireless#frequency">
    <rdfs:isDefinedBy rdf:resource="http://www.science.uva.nl/research/sne/schema/wireless.rdf"/>
    <rdfs:label xml:lang="en">frequency</rdfs:label>
    <rdfs:comment xml:lang="en">The central frequency of the channel at which an Interface operates, in Hz. For 802.11g, allowed values are 2412E6, 2417E6, 2422E6, 2427E6, 2432E6, 2437E6, 2442E6, 2447E6, 2452E6, 2457E6, 2462E6, 2467E6, 2472E6. Other standards have other frequencies.</rdfs:comment>
    <rdfs:domain rdf:resource="http://www.science.uva.nl/research/sne/ndl#ConnectionPoint"/>
    <rdfs:domain rdf:resource="http://www.science.uva.nl/research/sne/ndl/wireless#IEEE802-11NetworkElement"/>
    <rdfs:range rdf:resource="http://www.w3.org/2001/XMLSchema#float"/>
</rdf:Property>

<rdf:Property rdf:about="http://www.science.uva.nl/research/sne/ndl/wireless#encryption">
    <rdfs:isDefinedBy rdf:resource="http://www.science.uva.nl/research/sne/schema/wireless.rdf"/>
    <rdfs:label xml:lang="en">encryption</rdfs:label>
    <rdfs:comment xml:lang="en">The standard describing the initial authentication and key exchange used on a wireless network.</rdfs:comment>
    <rdfs:domain rdf:resource="http://www.science.uva.nl/research/sne/ndl#ConnectionPoint"/>
    <rdfs:domain rdf:resource="http://www.science.uva.nl/research/sne/ndl/wireless#IEEE802-11NetworkElement"/>
    <rdfs:range rdf:resource="http://www.science.uva.nl/research/sne/ndl/wireless#AccessSecurity"/>
</rdf:Property>

<!-- Adaptations -->

<layer:AdaptationProperty rdf:about="http://www.science.uva.nl/research/sne/ndl/wireless#Ethernet-in-802-11">
    <rdfs:isDefinedBy rdf:resource="http://www.science.uva.nl/research/sne/schema/wireless.rdf"/>
    <rdfs:label xml:lang="en">Ethernet in 802.11</rdfs:label>
    <rdfs:comment xml:lang="en">Adaptation of Ethernet in a specific SSID.</rdfs:comment>
    <rdf:type rdf:resource="http://www.w3.org/1999/02/22-rdf-syntax-ns#Property"/>
    <rdfs:range rdf:resource="http://www.science.uva.nl/research/sne/ndl#ConnectionPoint"/>
    <rdfs:range rdf:resource="http://www.science.uva.nl/research/sne/ndl/ethernet#EthernetNetworkElement"/> <!-- client layer -->
    <rdfs:domain rdf:resource="http://www.science.uva.nl/research/sne/ndl#ConnectionPoint"/>
    <rdfs:domain rdf:resource="http://www.science.uva.nl/research/sne/ndl/wireless#IEEE802-11NetworkElement"/> <!-- server layer -->
    <layer:clientCount rdf:datatype="http://www.w3.org/2001/XMLSchema#integer">1</layer:clientCount>
    <layer:serverCount rdf:datatype="http://www.w3.org/2001/XMLSchema#integer">1</layer:serverCount>
</layer:AdaptationProperty>
<layer:Layer rdf:about="http://www.science.uva.nl/research/sne/ndl/ethernet#EthernetNetworkElement"/>

</rdf:RDF>
